\documentclass[aspectratio=43]{beamer}
\usepackage[utf8]{inputenc}
\usepackage[T1]{fontenc}
\usepackage[brazil]{babel}
%\usepackage{tikz}
\usepackage{graphics,amssymb,amsfonts,amsmath}
%\usepackage{amstext}
%\usepackage{amssymb}
%\usepackage{stmaryrd}
%\usepackage{fullpage}
\usepackage{amsmath,amsfonts,amssymb,amsthm}
\usepackage{proof}
\usepackage{color}
\usepackage{listings}
\usepackage{setspace}
\usepackage{color}


\usetheme{CambridgeUS}
% \usetheme{Pittsburgh}
\usecolortheme{beaver}
\usefonttheme[onlymath]{serif}
\beamertemplatenavigationsymbolsempty

% Colocando numero de paginas no slide
%\setbeamertemplate{footline}[frame number]

\newcommand{\ria}{$\rightarrow$}
\newcommand{\Ria}{$\Rightarrow$}
\newcommand{\fall}{$\forall$}
\newcommand{\ex}{$\exists$}
\newcommand{\nao}{$\neg$}
\newcommand{\nex}{\nao\ex}
\newcommand{\nfall}{\nao\fall}
\newcommand{\andd}{$\wedge$}
\newcommand{\orr}{$\vee$}
\newcommand{\gam}{$\Gamma$}

\title[\sc{Resolu\c c\~ao}]{Resolu\c c\~ao 3.9}
\author[Guilherme Baumgratz Figueiroa]{Guilherme Baumgratz Figueiroa}
\institute[UFOP]{Universidade Federal de Ouro Preto} % opcional
\date{}

\begin{document}
	
	\begin{frame}
		\titlepage
	\end{frame}
	
	\section{Exercic\'io 9}
	
	\begin{frame}%\frametitle{Exercic\'io}
    
    	\begin{enumerate}[1.]
			\item Prove os seguintes sequentes usando dedu\c c\~ao natural: \\
		\end{enumerate}
				
	\end{frame}
    \subsection{b)}
    
	\begin{frame}[fragile]
    	
    	\begin{enumerate}[b)]
			
			\item $\{$ \fall P(x)\ria \nao Q(x) $\}$ $\vdash$ \nex  x.P(x)\ \andd\ Q(x) \\ 
			
		\end{enumerate}
        \vspace{100pt}
        \[
        \begin{array}{c}
		
        	\infer[_{}]
            {$\nex$  x. P(x)\ $\andd$\ Q(x)}
            {}
        
		\end{array}
        \]
        
	\end{frame}
    
    \begin{frame}[fragile]
    	
    	\begin{enumerate}[b)]
			
			\item $\{$ \fall P(x)\ria \nao Q(x) $\}$ $\vdash$ \nex  x.P(x)\ \andd\ Q(x) \\ 
			
		\end{enumerate}
        \textcolor{red}{\{\nex  x. P(x)\ \andd\ Q(x)\}}
        \vspace{95pt}
        \[
        \begin{array}{c}
		
        	\infer[_{(\textcolor{red}{Contr})}]
            {$\nex$  x. P(x)\ $\andd$\ Q(x)}
            {\textcolor{red}{\bot}}
        
		\end{array}
        \]
        
	\end{frame}
    
    \begin{frame}[fragile]
    	
    	\begin{enumerate}[b)]
			
			\item $\{$ \fall P(x)\ria \nao Q(x) $\}$ $\vdash$ \nex  x.P(x)\ \andd\ Q(x) \\ 
			
		\end{enumerate}
        \{\nex  x. P(x)\ \andd\ Q(x)\}
        \vspace{95pt}
        \[
        \begin{array}{c}
		
        	\infer[_{(Contr)}]
            {$\nex$  x. P(x)\ $\andd$\ Q(x)}
            {\infer[_{(\textcolor{red}{\land-I})}] 
            	{\bot}
                { \textcolor{red}{ Q(b) \hspace{35pt} \neg Q(b)}}
        	}
		\end{array}
        \]
        
	\end{frame}
    
    \begin{frame}[fragile]
    	
    	\begin{enumerate}[b)]
			
			\item $\{$ \fall P(x)\ria \nao Q(x) $\}$ $\vdash$ \nex  x.P(x)\ \andd\ Q(x) \\ 
			
		\end{enumerate}
        \{\nex  x. P(x)\ \andd\ Q(x)\}
        \vspace{100pt}
        \[
        \begin{array}{c}
		
        	\infer[_{(Contr)}]
            {$\nex$  x. P(x)\ $\andd$\ Q(x)}
            {\infer[_{(And-I)}] 
            	{\bot}
                {\infer[_{()}]
                	{Q(b)}
                    {\textcolor{red}{I}}
                \hspace{35pt} 
                \infer[_{()}]
                	{$\nao$Q(b)}
                    {\textcolor{red}{II}}
                }
        	}
		\end{array}
        \]
        
	\end{frame}
    
    \subsection{b) (I)}
    
    \begin{frame}[fragile]
    	
    	\begin{enumerate}[b)]
			
			\item $\{$ \fall P(x)\ria \nao Q(x) $\}$ $\vdash$ \nex  x.P(x)\ \andd\ Q(x) \\ 
			
		\end{enumerate}
        \{\nex  x. P(x)\ \andd\ Q(x)\}
        \vspace{100pt}
        \[
        \begin{array}{c}
		
        	\textcolor{red}{
            \infer[_{()}]
            {Q(b)}
            {}
            }
		\end{array}
        \]
        
	\end{frame}
    
    \begin{frame}[fragile]
    	
    	\begin{enumerate}[b)]
			
			\item $\{$ \fall P(x)\ria \nao Q(x) $\}$ $\vdash$ \nex  x.P(x)\ \andd\ Q(x) \\ 
			
		\end{enumerate}
        \{\nex  x. P(x)\ \andd\ Q(x)\}
        \vspace{95pt}
        \[
        \begin{array}{c}
		
        	\infer[_{(\textcolor{red}{\land-E})}]
            {Q(b)}
            {\textcolor{red}{P(b)\ \wedge \ Q(b)}}
		\end{array}
        \]
        
	\end{frame}
    
    \begin{frame}[fragile]
    	
    	\begin{enumerate}[b)]
			
			\item $\{$ \fall P(x)\ria \nao Q(x) $\}$ $\vdash$ \nex  x.P(x)\ \andd\ Q(x) \\ 
			
		\end{enumerate}
        \{\nex  x. P(x)\ \andd\ Q(x)\}
        \vspace{90pt}
        \[
        \begin{array}{c}
		
        	\infer[_{(\land-E)}]
            {Q(b)}
            {\infer[_{(\textcolor{red}{\exists-E})}]
                {P(b)\ $\andd$\ Q(b)}
            	{\textcolor{red}{\exists x.P(x)\ \wedge\ Q(x)}}
            }
		\end{array}
        \]
        
	\end{frame}
    
    \subsection{b) (II)}
    
    \begin{frame}[fragile]
    	
    	\begin{enumerate}[b)]
			
			\item $\{$ \fall P(x)\ria \nao Q(x) $\}$ $\vdash$ \nex  x.P(x)\ \andd\ Q(x) \\ 
			
		\end{enumerate}
        \{\nex  x. P(x)\ \andd\ Q(x)\}
        \vspace{100pt}
        \[
        \begin{array}{c}
		
        	\textcolor{red}{
            \infer[_{()}]
            {$\nao$ Q(b)}
            {}
            }
		\end{array}
        \]
        
	\end{frame}
    
    \begin{frame}[fragile]
    	
    	\begin{enumerate}[b)]
			
			\item $\{$ \fall P(x)\ria \nao Q(x) $\}$ $\vdash$ \nex x.P(x)\ \andd\ Q(x) \\ 
			
		\end{enumerate}
        \{\nex  x. P(x)\ \andd\ Q(x)\}
        \vspace{95pt}
        \[
        \begin{array}{c}
		
        	\infer[_{(\textcolor{red}{\to-E})}]
            {$\nao$ Q(b)}
            {\textcolor{red}{
            P(b) \rightarrow \neg Q(b) 
            \hspace{35pt}
            P(b)
            }
            }
		\end{array}
        \]
        
	\end{frame}
    
    \begin{frame}[fragile]
    	
    	\begin{enumerate}[b)]
			
			\item $\{$ \fall P(x)\ria \nao Q(x) $\}$ $\vdash$ \nex  x.P(x)\ \andd\ Q(x) \\ 
			
		\end{enumerate}
        \{\nex  x. P(x)\ \andd\ Q(x)\}
        \vspace{90pt}
        \[
        \begin{array}{c}
		
        	\infer[_{(\to-E)}]
            {$\nao$ Q(b)}
            {\infer[_{(\textcolor{red}{\forall-E})}] 
            	{P(b) $\ria$ $\nao$ Q(b)}
               	{\textcolor{red}{\forall x.P(x)\rightarrow \neg Q(x)}} 
            P(b)
            }
		\end{array}
        \]
        
	\end{frame}
    
    \begin{frame}[fragile]
    	
    	\begin{enumerate}[b)]
			
			\item $\{$ \fall P(x)\ria \nao Q(x) $\}$ $\vdash$ \nex  x.P(x)\ \andd\ Q(x) \\ 
			
		\end{enumerate}
        \{\nex  x. P(x)\ \andd\ Q(x)\}
        \vspace{90pt}
        \[
        \begin{array}{c}
		
        	\infer[_{(\to-E)}]
            {$\nao$ Q(b)}
            {\infer[_{(\forall-E)}] 
            	{P(b) $\ria$ $\nao$ Q(b)}
               	{$\fall$x.P(x)$\ria$ $\nao$ Q(x)} 
            \infer[_{(\textcolor{red}{\land-E})}] 
                {P(b)} 
                {\textcolor{red}{P(b)\ \wedge\ Q(b)}}
            }
		\end{array}
        \]
        
	\end{frame}
    
    \begin{frame}[fragile]
    	
    	\begin{enumerate}[b)]
			
			\item $\{$ \fall P(x)\ria \nao Q(x) $\}$ $\vdash$ \nex  x.P(x)\ \andd\ Q(x) \\ 
			
		\end{enumerate}
        \{\nex  x. P(x)\ \andd\ Q(x)\}
        \vspace{90pt}
        \[
        \begin{array}{c}
		
        	\infer[_{(\to-E)}]
            {$\nao$ Q(b)}
            {\infer[_{(\forall-E)}] 
            	{P(b) $\ria$ $\nao$ Q(b)}
               	{$\fall$x.P(x)$\ria$ $\nao$ Q(x)} 
            \infer[_{(\land-E)}] 
                {P(b)} 
                {\infer[_{(\textcolor{red}{\exists-E})}] 
                        	{P(b)\ $\andd$\ Q(b)}
                        	{\textcolor{red}{\exists x.P(x)\ \wedge\ Q(x)}}
                }
            }
		\end{array}
        \]
        
	\end{frame}
    
    \subsection{b)}
        
	\begin{frame}[fragile]
    
    	\begin{enumerate}[b)]
			
			\item $\{$ \fall P(x)\ria \nao Q(x) $\}$ $\vdash$ \nex  x.P(x)\ \andd\ Q(x) \\ 
			
		\end{enumerate}
        \vspace{50pt}
		\[
        \begin{array}{c}
		\infer[_{(C)}]
			{$\nex$ x.P(x)\ $\andd$\ Q(x)}
			{\infer[_{(\land-I)}] 
            	{\bot}
                {\infer[_{(\land-E)}] 
                	{Q(b)}
                    {\infer[_{(\exists-E)}]
                    	{P(b)\ $\andd$\ Q(b)}
                        {$\ex$x.P(x)\ $\andd$\ Q(x)}
                    }
                \infer[_{(\to-E)}] 
                	{$\nao$ Q(b)}
                	{\infer[_{(\forall-E)}] 
                    	{P(b) $\ria$ $\nao$ Q(b)}
                    	{$\fall$x.P(x)$\ria$ $\nao$ Q(x)}
                    \infer[_{(\land-E)}] 
                    	{P(b)}
                        {\infer[_{(\exists-E)}] 
                        	{P(b)\ $\andd$\ Q(b)}
                        	{$\ex$x.P(x)\ $\andd$\ Q(x)}
                        }
                    }
                }
            }
		\end{array}
        \]
		
	\end{frame}
	
\end{document}

